src/Compilers/Z/Bounds/MapCastByDeBruijnInterp.v
@@ -14,15 +14,15 @@ Require Import Crypto.Util.PointedProp.
 
 Lemma MapCastCorrect
       {round_up}
-      {t} (e : Expr base_type op t)
+      {t} (e : Expr t)
       (Hwf : Wf e)
       (input_bounds : interp_flat_type Bounds.interp_base_type (domain t))
   : forall {b} e' (He':MapCast round_up e input_bounds = Some (existT _ b e'))
            v v' (Hv : Bounds.is_bounded_by input_bounds v /\ cast_back_flat_const v' = v)
            (Hside : to_prop (InterpSideConditions e v)),
-    Interp (@Bounds.interp_op) e input_bounds = b
-    /\ Bounds.is_bounded_by b (Interp interp_op e v)
-    /\ cast_back_flat_const (Interp interp_op e' v') = (Interp interp_op e v).
+    Compilers.Syntax.Interp (@Bounds.interp_op) e input_bounds = b
+    /\ Bounds.is_bounded_by b (Compilers.Syntax.Interp interp_op e v)
+    /\ cast_back_flat_const (Compilers.Syntax.Interp interp_op e' v') = (Compilers.Syntax.Interp interp_op e v).
 Proof.
   apply MapCastCorrect; auto.
   { apply is_bounded_by_interp_op. }
@@ -31,18 +31,18 @@ Qed.
 
 Lemma MapCastCorrect_eq
       {round_up}
-      {t} (e : Expr base_type op t)
+      {t} (e : Expr t)
       {evb ev}
       (Hwf : Wf e)
       (input_bounds : interp_flat_type Bounds.interp_base_type (domain t))
   : forall {b} e' (He':MapCast round_up e input_bounds = Some (existT _ b e'))
            v v' (Hv : Bounds.is_bounded_by input_bounds v /\ cast_back_flat_const v' = v)
            (Hside : to_prop (InterpSideConditions e v))
-           (Hevb : evb = Interp (@Bounds.interp_op) e input_bounds)
-           (Hev : ev = Interp interp_op e v),
+           (Hevb : evb = Compilers.Syntax.Interp (@Bounds.interp_op) e input_bounds)
+           (Hev : ev = Compilers.Syntax.Interp interp_op e v),
     evb = b
     /\ Bounds.is_bounded_by b ev
-    /\ cast_back_flat_const (Interp interp_op e' v') = ev.
+    /\ cast_back_flat_const (Compilers.Syntax.Interp interp_op e' v') = ev.
 Proof.
   intros; subst; apply MapCastCorrect; auto.
 Qed.
