src/Compilers/Z/InlineInterp.v
@@ -4,12 +4,12 @@ Require Import Crypto.Compilers.InlineInterp.
 Require Import Crypto.Compilers.Z.Syntax.
 Require Import Crypto.Compilers.Z.Inline.
 
-Definition InterpInlineConstAndOpp {interp_base_type interp_op} {t} (e : Expr base_type op t) (Hwf : Wf e)
-  : forall x, Interp interp_op (InlineConstAndOpp e) x = Interp interp_op e x
+Definition InterpInlineConstAndOpp {interp_base_type interp_op} {t} (e : Expr t) (Hwf : Wf e)
+  : forall x, Compilers.Syntax.Interp interp_op (InlineConstAndOpp e) x = Compilers.Syntax.Interp interp_op e x
   := @InterpInlineConst _ interp_base_type _ _ _ t e Hwf.
 
-Definition InterpInlineConst {interp_base_type interp_op} {t} (e : Expr base_type op t) (Hwf : Wf e)
-  : forall x, Interp interp_op (InlineConst e) x = Interp interp_op e x
+Definition InterpInlineConst {interp_base_type interp_op} {t} (e : Expr t) (Hwf : Wf e)
+  : forall x, Compilers.Syntax.Interp interp_op (InlineConst e) x = Compilers.Syntax.Interp interp_op e x
   := @InterpInlineConst _ interp_base_type _ _ _ t e Hwf.
 
 Hint Rewrite @InterpInlineConstAndOpp @InterpInlineConst using solve_wf_side_condition : reflective_interp.
