src/Compilers/Z/InlineWf.v
@@ -4,11 +4,11 @@ Require Import Crypto.Compilers.InlineWf.
 Require Import Crypto.Compilers.Z.Syntax.
 Require Import Crypto.Compilers.Z.Inline.
 
-Definition Wf_InlineConstAndOpp {t} (e : Expr base_type op t) (Hwf : Wf e)
+Definition Wf_InlineConstAndOpp {t} (e : Expr t) (Hwf : Wf e)
   : Wf (InlineConstAndOpp e)
   := @Wf_InlineConst _ _ _ t e Hwf.
 
-Definition Wf_InlineConst {t} (e : Expr base_type op t) (Hwf : Wf e)
+Definition Wf_InlineConst {t} (e : Expr t) (Hwf : Wf e)
   : Wf (InlineConst e)
   := @Wf_InlineConst _ _ _ t e Hwf.
 
