src/Compilers/Z/InterpSideConditions.v
@@ -5,5 +5,5 @@ Require Import Crypto.Compilers.InterpSideConditions.
 Require Import Crypto.Util.PointedProp.
 Require Import Crypto.Util.Notations.
 
-Definition InterpSideConditions {t} (e : Expr base_type op t) : interp_flat_type interp_base_type (domain t) -> pointed_Prop
+Definition InterpSideConditions {t} (e : Expr t) : interp_flat_type interp_base_type (domain t) -> pointed_Prop
     := InterpSideConditions interp_op (@interped_op_side_conditions) e.
