src/Util/Notations.v
@@ -10,6 +10,10 @@ Require Export Crypto.Util.GlobalSettings.
 
 Reserved Notation "x -> y" (at level 99, right associativity, y at level 200).
 Reserved Notation "()" (at level 0).
+Reserved Infix "∘" (at level 40, left associativity).
+Reserved Infix "∘ᶠ" (at level 40, left associativity).
+Reserved Infix "∘f" (at level 40, left associativity).
+Reserved Infix "'o'" (at level 40, left associativity).
 Reserved Infix "=?" (at level 70, no associativity).
 Reserved Infix "<?" (at level 70, no associativity).
 Reserved Infix "<=?" (at level 70, no associativity).
