src/Compilers/Z/FoldTypes.v
@@ -7,11 +7,11 @@ Section min_or_max.
   Context (f : base_type -> base_type -> base_type)
           (init : base_type).
 
-  Definition TypeFold {t} (e : Expr base_type op t) : base_type
+  Definition TypeFold {t} (e : Expr t) : base_type
     := TypeFold (fun t => t) f init e.
 End min_or_max.
 
-Definition MaxTypeUsed {t} (e : Expr base_type op t) : base_type
+Definition MaxTypeUsed {t} (e : Expr t) : base_type
   := TypeFold base_type_max (TWord 0) e.
-Definition MinTypeUsed {t} (e : Expr base_type op t) : base_type
+Definition MinTypeUsed {t} (e : Expr t) : base_type
   := TypeFold base_type_min TZ e.
